examples/ecAdd/proofs/ecAdd_safety_cases.ec
@@ -7,34 +7,6 @@ require import EcAdd_spec.
 require import ExtraFacts Parameters.
      
 
-
-
-lemma nosmt mul_inj (a b r : int) : coprime r P
-    => a * r %% P = b * r %% P => a %% P = b %% P.
-move => coprime_h eq.
- have : a * r * (inv r) %% P = b * r * (inv r) %% P.
-  have ->: (a * r) * (inv r) %% P = (a * r %% P)  * (inv r) %% P.
-  smt(@IntDiv).
-  rewrite eq.
-  smt(@IntDiv).
-  have ->: a * r * inv r = a * (r * inv r). smt(@IntDiv).
-  have ->: b * r * inv r = b * (r * inv r). smt(@IntDiv).
-  have ->: a * (r * inv r) %% P = a * (r * inv r %% P) %% P.
-  smt(@IntDiv).
-  have ->: b * (r * inv r) %% P = b * (r * inv r %% P) %% P.
-  smt(@IntDiv).
-  rewrite inv_ax_opp. smt(@IntDiv).
-  simplify.
-  auto.
-qed.
-
-lemma nosmt mul_inj_contra_pos (a b r : int) :  coprime r P =>
-  a %% P <> b %% P =>  a * r %% P <> b * r %% P.
-proof. smt(mul_inj). qed.
-
-
-
-
 lemma ecAdd_safety_1 x1_in y1_in x2_in y2_in :  0 <= x1_in /\ 0 <= y1_in /\ 0 <= x2_in /\ 0 <= y2_in =>
  phoare[ AlmostYul.main : 
          arg = (x1_in,y1_in,x2_in,y2_in) /\
@@ -68,7 +40,7 @@ rewrite /as_bool.
 have ->: (x2{hr} * x2{hr} * x2{hr} * R + 3 * R)
  = (x2{hr} * x2{hr} * x2{hr}  + 3 ) * R. smt().
 apply mul_inj_contra_pos. smt. 
-smt. 
+smt. smt.
 inline 3. while (true). auto. auto. exfalso.
 rcondt 1. auto.
 seq 2 : (#pre  /\ func109 = (!p1IsInfinity /\ p2IsInfinity)). inline*.  wp. skip. auto.
@@ -82,7 +54,7 @@ ecall (pointIsInCurve_m_h x1 y1).  skip. progress.
 have ->: (x1{hr} * x1{hr} * x1{hr} * R + 3 * R)
  = (x1{hr} * x1{hr} * x1{hr}  + 3 ) * R. smt().
 apply mul_inj_contra_pos. smt.
- smt.
+ smt. smt. 
 seq 3 : (false). inline 3.
  while (true). auto. auto. exfalso.
 rcondt 1. auto.
@@ -105,12 +77,12 @@ inline 5. inline 4. wp.
 ecall (pointIsInCurve_m_h x2 y2).
 inline 2. wp.
 ecall (pointIsInCurve_m_h x1 y1).
-skip. progress. 
-have ->: (x1{hr} * x1{hr} * x1{hr} * R + 3 * R)
-  = (x1{hr} * x1{hr} * x1{hr} + 3) * R. smt().
+skip. progress.  
+(* have ->: (x1{hr} * x1{hr} * x1{hr} * R + 3 * R) *)
+(*   = (x1{hr} * x1{hr} * x1{hr} + 3) * R. smt(). *)
 have ->: (x2{hr} * x2{hr} * x2{hr} * R + 3 * R)
   = (x2{hr} * x2{hr} * x2{hr} + 3) * R. smt().
-have ok : ! pointIsInCurve x1{hr} y1{hr} \/ ! pointIsInCurve x2{hr} y2{hr} . smt.
+have ok : ! pointIsInCurve x2{hr} y1{hr} \/ ! pointIsInCurve x2{hr} y2{hr} . smt.
 have okk : coprime R P. smt.
 smt (mul_inj_contra_pos).
 seq 6 : (false).
@@ -125,9 +97,9 @@ ecall (into_m_h y1_in).
 ecall (into_m_h x1_in). skip. progress;smt().  
 seq 3 : (false).
 rcondt 3. inline 2. wp.  
-ecall (pointIsInCurve_m_h x1 y1). skip. progress. rewrite /as_bool.
-have ->: (x1{hr} * x1{hr} * x1{hr} * R + 3 * R) = (x1{hr} * x1{hr} * x1{hr}+ 3) * R. smt().
-apply mul_inj_contra_pos. smt. smt.
+ecall (pointIsInCurve_m_h x1 y1). skip. progress.
+have ->: (x2{hr} * x2{hr} * x2{hr} * R + 3 * R) = (x2{hr} * x2{hr} * x2{hr}+ 3) * R. smt().
+apply mul_inj_contra_pos. smt. smt. smt.
 inline 3. while (true). auto. auto. exfalso.
 rcondt 1. auto. simplify.
 seq 4 : ((((((((((
@@ -139,13 +111,13 @@ seq 4 : ((((((((((
           p1IsInfinity = pIsInfinity (x1_in, y1_in) /\
           p2IsInfinity = pIsInfinity (x2_in, y2_in)) /\
          func43 = (p1IsInfinity /\ !p2IsInfinity)) /\
-        ! as_bool func43) /\
+        ! func43) /\
        func109 = (!p1IsInfinity /\ p2IsInfinity)) /\
-      ! as_bool func109) /\
+      ! func109) /\
      func211 = (x1_in = x2_in /\ func219)) /\
-    ! as_bool func211) /\
+    ! func211) /\
    func325 = (x1_in = x2_in /\ y1_in = y2_in)) /\
-  ! as_bool func325 /\ x1 = x1_in * R %% P /\ y1 = y1_in * R %% P /\ x2 = x2_in * R %% P /\ y2 = y2_in * R %% P).  
+  ! func325 /\ x1 = x1_in * R %% P /\ y1 = y1_in * R %% P /\ x2 = x2_in * R %% P /\ y2 = y2_in * R %% P).  
 ecall (into_m_h y2_in).
 ecall (into_m_h x2_in).
 ecall (into_m_h y1_in).
@@ -162,15 +134,14 @@ have :  ! pointIsInCurve x1_in y1_in \/ ! pointIsInCurve x2_in y2_in. smt.
 elim. progress.
 left.
 have ->: (x1_in * x1_in * x1_in * R + 3 * R) = (x1_in * x1_in * x1_in + 3 ) * R. smt().
-apply mul_inj_contra_pos. smt. smt.
+apply mul_inj_contra_pos. smt. smt. smt.
 progress.
 right.
 have ->: (x2_in * x2_in * x2_in * R + 3 * R) = (x2_in * x2_in * x2_in + 3 ) * R. smt().
-apply mul_inj_contra_pos. smt.  smt.
+apply mul_inj_contra_pos. smt.  smt. smt.
 inline 6.
 while(true). auto. auto. exfalso.
 qed.  
-
  
   
 
