examples/ecAdd/proofs/gcd.ec
@@ -3,9 +3,8 @@ require import AllCore.
 require import IntDiv Int.
 require import Gcd_props.
 
-
-
 module GCDAlgs = {
+
   proc simplify_t(t:int) = {
       while (!odd t){
         t <- t %/ 2;
@@ -38,53 +37,33 @@ module GCDAlgs = {
     
 
 lemma simplify_divby2s t_in :
-   phoare [ GCDAlgs.simplify_t : t = t_in /\ t <> 0 ==> res = div_by2s t_in ] = 1%r.
+   phoare [ GCDAlgs.simplify_t : t = t_in /\ t <> 0 
+                     ==> res = div_by2s t_in ] = 1%r.
 proc.
 while (div_by2s t = div_by2s t_in /\ t <> 0) `|t|.
-progress.
-wp. skip. progress. smt. smt.
+progress. wp. skip. progress. smt. smt(@Int).
  case (t{hr} < 0). progress.
-    have ->: `|t{hr} %/ 2| = - (t{hr} %/ 2). smt.
-    have ->: `|t{hr}| = - (t{hr}). smt.
-    smt.
+    have ->: `|t{hr} %/ 2| = - (t{hr} %/ 2). smt(@Int).
+    have ->: `|t{hr}| = - (t{hr}). smt(@Int).
+    smt(@Int).
     progress.
-    have ->: `|t{hr} %/ 2| =  (t{hr} %/ 2). smt.
-    have ->: `|t{hr}| =  (t{hr}). smt.
-    smt.    
-skip. progress. smt. smt. 
+    have ->: `|t{hr} %/ 2| =  (t{hr} %/ 2). smt(@Int).
+    have ->: `|t{hr}| =  (t{hr}). smt(@Int).
+    smt(@Int).    
+skip. progress. smt(). smt.
 qed.    
 
 
 
-lemma main3_term : phoare [GCDAlgs.main3 : odd u /\ 0 < u /\ 0 < v ==> true ] = 1%r.
+lemma main3_term : phoare [GCDAlgs.main3 : odd u /\ 0 < u /\ 0 < v 
+                                                     ==> true ] = 1%r.
 proc. unroll 3.
 rcondt 3. wp. skip. progress. smt()    .
 while (t = u - v /\ !odd t /\ odd u /\ odd v /\ 0 < u /\ 0 < v) (max u v).
 progress.    
-wp. skip. progress.
-case (v{hr} < u{hr}). progress.
-    smt.
-    smt.
-    smt.
-    smt. smt. smt.
-pose x := div_by2s (u{hr} - v{hr}).     
-case (v{hr} < u{hr}). progress.
-have f1 : 0 < x < u{hr} - v{hr}. split. smt.  smt. 
-smt.
-    move => q.
- case (v{hr} <= x).
-   move => mh.
-      smt.
-progress.
-have f1 : 0 < -x < v{hr} - u{hr}. split. smt.    
-progress.
-     have : u{hr} - v{hr} < x. smt.
-    smt.
-    smt.    
-wp.    skip.
-progress.
-smt.
-    smt. smt. smt. smt. smt.
+wp. skip. progress;smt.
+wp. skip.
+progress;smt.
 qed.    
 
 
@@ -98,26 +77,19 @@ seq 4 : (gcd u_in v_in = gcd u v /\ odd u /\ odd v
   /\ 0 < u /\ 0 < v ).
 wp. skip. progress.
 have ->: 0 < div_by2s (-v{hr}) = false. smt(div_by2s1). simplify.
-smt.                            
-smt.
-smt. smt. smt.
-seq 1 : ((gcd u_in v_in = gcd t (if 0 < t then v else u) /\ !odd t /\ odd u /\ odd v)  /\  0 < u /\ 0 < v /\ t = u - v).
-wp. skip. progress.
-rewrite H. 
-smt.
-smt.
-while (gcd u_in v_in =  gcd t (if 0 < t then v else u) /\ !odd t /\ odd u /\ odd v /\  0 <= u /\ 0 <= v /\ t = u - v).
-seq 1 : (gcd u_in v_in =gcd t (if 0 < t then v else u) /\ odd t /\ odd u /\ odd v /\ t <> 0 /\ 0 <= u /\ 0 <= v /\ t = div_by2s (u - v)).
-wp. skip. progress. rewrite H. 
-smt.
-smt.
-smt.
+smt. smt. smt. smt. smt.
+seq 1 : ((gcd u_in v_in = gcd t (if 0 < t then v else u) 
+             /\ !odd t /\ odd u /\ odd v)  /\  0 < u /\ 0 < v /\ t = u - v).
+wp. skip. progress;smt.
+while (gcd u_in v_in =  gcd t (if 0 < t then v else u) 
+              /\ !odd t /\ odd u /\ odd v /\  0 <= u /\ 0 <= v /\ t = u - v).
+seq 1 : (gcd u_in v_in =gcd t (if 0 < t then v else u) 
+             /\ odd t /\ odd u /\ odd v /\ t <> 0 /\ 0 <= u 
+             /\ 0 <= v /\ t = div_by2s (u - v)).
+wp. skip. progress;smt.
 seq 1 : (gcd u_in v_in = gcd t (if 0 < t then v else u) /\ odd t /\ odd u /\ odd v /\ t <> 0
    /\ (u = if 0 < t then t else u) /\ (v = if 0 < t then v else -t) /\ 0 <= u /\ 0 <= v).
-wp. skip. progress.
-rewrite H. 
-case (0 < t{hr}). auto.
-auto. smt. smt. smt. smt. smt. smt. smt. smt.  
+wp. skip. progress;smt.
 wp. skip. progress.
 rewrite H. 
 case (0 < t{hr}). auto.
@@ -126,25 +98,25 @@ progress. rewrite H8. simplify.
 rewrite gcd6. smt.
 rewrite H5.
 progress. rewrite H8. simplify. smt. smt.
-skip. progress. smt. smt. smt.
+skip. progress;smt.
 qed.
 
 
-lemma main3_correct_and_terminating u_in v_in : phoare [ GCDAlgs.main3 : arg = (u_in, v_in) /\ 0 < u_in /\ 0 < v_in /\ odd u ==> res = gcd u_in v_in ] = 1%r.
+lemma main3_correct_and_terminating u_in v_in :
+ phoare [ GCDAlgs.main3 : arg = (u_in, v_in) /\ 0 < u_in /\ 0 < v_in /\ odd u 
+           ==> res = gcd u_in v_in ] = 1%r.
 phoare split ! 1%r 0%r. smt().
-conseq main3_term. smt().
-    hoare. simplify.
+conseq main3_term. smt(). hoare. simplify.
 apply gcd_odd_alg.
 qed.    
 
 
-lemma main3_main4 u_in v_in : equiv [ GCDAlgs.main3 ~ GCDAlgs.main4 : arg{1} = (u_in, v_in) /\ 0 < u_in /\ 0 < v_in
- /\ odd u_in /\ ={arg} ==> ={res} ].
+lemma main3_main4 u_in v_in :
+ equiv [ GCDAlgs.main3 ~ GCDAlgs.main4 : arg{1} = (u_in, v_in) /\ 0 < u_in /\ 0 < v_in
+               /\ odd u_in /\ ={arg} ==> ={res} ].
 proc.
 seq 2 2 : (={t,u,v}).
 wp. skip. progress.
-(* ecall {2} (simplify_divby2s v{2}). wp. *)
-(* skip. progress. smt. *)
 while (={t,u,v}). wp.
 ecall {2} (simplify_divby2s t{2}). wp.
 skip. progress. skip. progress.
@@ -152,7 +124,9 @@ qed.
 
 
 
-lemma main4_correct_and_terminating u_in v_in : phoare [ GCDAlgs.main4 : arg = (u_in, v_in) /\ 0 < u_in /\ 0 < v_in /\ odd u ==> res = gcd u_in v_in ] = 1%r.
+lemma main4_correct_and_terminating u_in v_in :
+   phoare [ GCDAlgs.main4 : arg = (u_in, v_in) /\ 0 < u_in /\ 0 < v_in /\ odd u 
+               ==> res = gcd u_in v_in ] = 1%r.
 bypr.
 progress.
  have <-: Pr[GCDAlgs.main3(u{m}, v{m}) @ &m : res = gcd u_in v_in] = 1%r.
